revm: add an explicit definition of logical operators to handle more cases

CoqOfRust/ruint/links/macros.v
@@ -4,6 +4,16 @@ Require Import core.ops.links.arith.
 Require Import ruint.links.lib.
 Require Import ruint.macros.
 
+Module Impl_Div_for_Uint_Uint.
+  Definition Self (BITS LIMBS : Usize.t) : Set :=
+    Uint.t BITS LIMBS.
+
+  Instance run (BITS LIMBS : Usize.t) :
+    Div.Run (Self BITS LIMBS) (Uint.t BITS LIMBS) (Uint.t BITS LIMBS).
+  Admitted.
+End Impl_Div_for_Uint_Uint.
+Export Impl_Div_for_Uint_Uint.
+
 Module Impl_Rem_for_Uint_Uint.
   Definition Self (BITS LIMBS : Usize.t) : Set :=
     Uint.t BITS LIMBS.
